share and gather

qstar/src/QStarRef.fst
@@ -9,9 +9,9 @@ let core_ref = P.ref _ qstar_heap_pcm
 //All the qubits are stores in this ref cell
 assume
 val qstar_state : core_ref
-
-let pts_to (qs:qbits) (state:qvec qs) : vprop =
-  exists_ (fun perm -> P.pts_to qstar_state ({frac=Some perm; qs; state}))
+let pperm = p:perm {p `lesser_equal_perm` full_perm}
+let pts_to (qs:qbits) ([@@@smt_fallback]state:qvec qs) : vprop =
+  exists_ (fun (perm:pperm) -> P.pts_to qstar_state ({frac=Some perm; qs; state}))
 
 let apply_gate (qs:qbits) (#state:qvec qs) (gate:qvec qs -> qvec qs)
   : STT unit
@@ -20,14 +20,48 @@ let apply_gate (qs:qbits) (#state:qvec qs) (gate:qvec qs -> qvec qs)
   = let perm = elim_exists () in
     P.upd_gen qstar_state ({frac=Some (Ghost.reveal perm); qs; state}) ({frac=Some (Ghost.reveal perm); qs;state=gate state})
       (QStarHeap.apply_fpupd #qs #perm #state gate);
-    intro_exists_erased perm (fun perm -> P.pts_to qstar_state ({frac=Some perm; qs; state=gate state}))
+    intro_exists_erased #pperm perm (fun perm -> P.pts_to qstar_state ({frac=Some perm; qs; state=gate state}))
+
+let split_perm (p:pperm)
+  : c:pperm{ composable_frac_opt (Some c) (Some c) }
+  = half_perm p
+
+let intro_pts_to #o (#p:pperm) qs #s ()
+  : STGhostT unit o
+    (P.pts_to qstar_state ({frac = Some p; qs; state=s}))
+    (fun _ -> pts_to qs s)
+  = intro_exists #pperm p (fun p -> P.pts_to qstar_state ({frac = Some p; qs; state=s}));
+    ()
 
 let share (#o:_) (qs:qbits) (qs':qbits{ disjoint_qbits qs qs'}) (#state:qvec qs) (#state':qvec qs')
   : STGhostT unit o
     (pts_to (qs `OrdSet.union` qs')
             (state `tensor` state'))
     (fun _ -> pts_to qs state `star` pts_to qs' state')
-  = admit_()
+  = let perm = elim_exists #pperm () in
+    P.share qstar_state _
+      ({ frac = Some (Ghost.reveal (half_perm perm));
+               qs = qs;
+               state = state })
+      ({ frac = Some (Ghost.reveal (half_perm perm));
+               qs = qs';
+               state = state' });
+    intro_pts_to qs ();
+    intro_pts_to qs' ()
+
+
+let gather (#o:_) (qs:qbits) (qs':qbits{ disjoint_qbits qs qs'}) (#state:qvec qs) (#state':qvec qs')
+  : STGhostT unit o
+    (pts_to qs state `star` pts_to qs' state')
+    (fun _ -> pts_to (qs `OrdSet.union` qs') (state `tensor` state'))
+  = let perm = elim_exists #pperm #_ #(fun pperm -> P.pts_to qstar_state ({frac = Some pperm; qs; state})) () in
+    let perm' = elim_exists #pperm #_ #(fun pperm -> P.pts_to qstar_state ({frac = Some pperm; qs=qs'; state=state'})) () in
+    P.gather qstar_state ({frac = Some (Ghost.reveal perm); qs; state})
+                         ({frac = Some (Ghost.reveal perm'); qs=qs'; state=state'});
+    rewrite (P.pts_to qstar_state _)
+            (P.pts_to qstar_state ({frac=Some (sum_perm perm perm'); qs=(qs `OrdSet.union` qs'); state=(state `tensor` state')}));
+    intro_pts_to _ ()
+
 
 let single (q:qbit) : qbits = OrdSet.singleton q
 let singleton q (b:bool) : qvec (single q) = admit()
